Add factrial runtime

examples/fact_main.erl
@@ -1,0 +1,18 @@
+-module(fact_main).
+-export([fact/1]).
+
+fact(N) ->
+    _ = spawn(factorial, factorial_system, [int2nat(N), self()]),
+    receive
+        {nat_msg, Result} ->
+            io:fwrite("fact(~w) = ~w~n", [N, nat2int(Result)]);
+        _ ->
+            io:fwrite("error~n")
+    end.
+
+nat2int({o}) -> 0;
+nat2int({s, N}) -> nat2int(N) + 1.
+
+int2nat(0) -> {o};
+int2nat(N) when N > 0 -> {s, int2nat(N - 1)};
+int2nat(_) -> {o}.
